Translation/SAst.v
@@ -10,7 +10,7 @@ Inductive sterm : Type :=
 | sSort (s : sort)
 | sProd (nx : name) (A B : sterm)
 | sLambda (nx : name) (A B t : sterm)
-| sApp (u : sterm) (nx : name) (A B v : sterm)
+| sApp (u A B v : sterm)
 (* Homogenous equality *)
 | sEq (A u v : sterm)
 | sRefl (A u : sterm)
