Translation/SCommon.v
@@ -3,18 +3,9 @@ From Equations Require Import Equations DepElimDec.
 From Template Require Import Ast utils Typing.
 From Translation Require Import util SAst SInduction SLiftSubst.
 
-Record scontext_decl := { sdecl_name : name ;
-                          sdecl_body : option sterm ;
-                          sdecl_type : sterm }.
+Definition scontext := list sterm.
 
-Definition svass x A :=
-  {| sdecl_name := x; sdecl_body := None; sdecl_type := A |}.
-Definition svdef x t A :=
-  {| sdecl_name := x; sdecl_body := Some t; sdecl_type := A |}.
-
-Definition scontext := (list scontext_decl).
-
-Definition ssnoc (Γ : scontext) (d : scontext_decl) := d :: Γ.
+Definition ssnoc (Γ : scontext) (d : sterm) := d :: Γ.
 
 Notation " Γ ,, d " := (ssnoc Γ d) (at level 20, d at next level) : s_scope.
 Delimit Scope s_scope with s.
@@ -94,11 +85,11 @@ Proof.
 Defined.
 
 Lemma eq_safe_nth :
-  forall {Γ n x A isdecl isdecl'},
-    safe_nth (Γ ,, svass x A) (exist _ (S n) isdecl') =
+  forall {Γ n A isdecl isdecl'},
+    safe_nth (Γ ,, A) (exist _ (S n) isdecl') =
     safe_nth Γ (exist _ n isdecl).
 Proof.
-  intros Γ n x A isdecl isdecl'.
+  intros Γ n A isdecl isdecl'.
   apply eq_safe_nth'.
 Defined.
 
@@ -312,43 +303,18 @@ Defined.
 
 (* Lifting of context *)
 
-Definition lift_decl n k d : scontext_decl :=
-  {| sdecl_name := sdecl_name d ;
-     sdecl_body := option_map (lift n k) (sdecl_body d) ;
-     sdecl_type := lift n k (sdecl_type d)
-  |}.
-
 Fixpoint lift_context n Γ : scontext :=
   match Γ with
   | nil => nil
-  | A :: Γ => (lift_decl n #|Γ| A) :: (lift_context n Γ)
+  | A :: Γ => (lift n #|Γ| A) :: (lift_context n Γ)
   end.
-
-Fact lift_decl0 :
-  forall {d k}, lift_decl 0 k d = d.
-Proof.
-  intros d k.
-  destruct d as [x b A].
-  unfold lift_decl. cbn. rewrite lift00. f_equal.
-  destruct b.
-  - cbn. rewrite lift00. reflexivity.
-  - reflexivity.
-Defined.
 
 Fact lift_context0 :
   forall {Γ}, lift_context 0 Γ = Γ.
 Proof.
   intro Γ. induction Γ.
   - reflexivity.
-  - cbn. rewrite lift_decl0. rewrite IHΓ. reflexivity.
-Defined.
-
-Fact lift_decl_svass :
-  forall na A n k,
-    lift_decl n k (svass na A) = svass na (lift n k A).
-Proof.
-  intros na A n k.
-  reflexivity.
+  - cbn. rewrite lift00. rewrite IHΓ. reflexivity.
 Defined.
 
 Fact lift_context_length :
@@ -362,8 +328,8 @@ Defined.
 
 Fact safe_nth_lift_context :
   forall {Γ Δ : scontext} {n isdecl isdecl'},
-    sdecl_type (safe_nth (lift_context #|Γ| Δ) (exist _ n isdecl)) =
-    lift #|Γ| (#|Δ| - n - 1) (sdecl_type (safe_nth Δ (exist _ n isdecl'))).
+    safe_nth (lift_context #|Γ| Δ) (exist _ n isdecl) =
+    lift #|Γ| (#|Δ| - n - 1) (safe_nth Δ (exist _ n isdecl')).
 Proof.
   intros Γ Δ. induction Δ.
   - cbn. easy.
@@ -374,8 +340,8 @@ Defined.
 
 Fact lift_context_ex :
   forall {Δ Ξ : scontext} {n isdecl isdecl'},
-    lift0 (S n) (sdecl_type (safe_nth (lift_context #|Δ| Ξ) (exist _ n isdecl))) =
-    lift #|Δ| #|Ξ| (lift0 (S n) (sdecl_type (safe_nth Ξ (exist _ n isdecl')))).
+    lift0 (S n) (safe_nth (lift_context #|Δ| Ξ) (exist _ n isdecl)) =
+    lift #|Δ| #|Ξ| (lift0 (S n) (safe_nth Ξ (exist _ n isdecl'))).
 Proof.
   intros Δ Ξ n isdecl isdecl'.
   erewrite safe_nth_lift_context.
@@ -395,25 +361,11 @@ Defined.
 
 (* Substitution in context *)
 
-Definition subst_decl n u d : scontext_decl :=
-  {| sdecl_name := sdecl_name d ;
-     sdecl_body := option_map (subst u n) (sdecl_body d) ;
-     sdecl_type := (sdecl_type d){ n := u }
-  |}.
-
 Fixpoint subst_context u Δ :=
   match Δ with
   | nil => nil
-  | A :: Δ => (subst_decl #|Δ| u A) :: (subst_context u Δ)
+  | A :: Δ => (A{ #|Δ| := u }) :: (subst_context u Δ)
   end.
-
-Fact subst_decl_svass :
-  forall na A n u,
-    subst_decl n u (svass na A) = svass na (A{ n := u }).
-Proof.
-  intros na A n u.
-  reflexivity.
-Defined.
 
 Fact subst_context_length :
   forall {u Ξ}, #|subst_context u Ξ| = #|Ξ|.
@@ -426,8 +378,8 @@ Defined.
 
 Fact safe_nth_subst_context :
   forall {Δ : scontext} {n u isdecl isdecl'},
-    sdecl_type (safe_nth (subst_context u Δ) (exist _ n isdecl)) =
-    (sdecl_type (safe_nth Δ (exist _ n isdecl'))) { #|Δ| - S n := u }.
+    (safe_nth (subst_context u Δ) (exist _ n isdecl)) =
+    (safe_nth Δ (exist _ n isdecl')) { #|Δ| - S n := u }.
 Proof.
   intro Δ. induction Δ.
   - cbn. easy.
