Translation/util.v
@@ -116,3 +116,20 @@ Tactic Notation "erewrite_assumption" "by" tactic(tac) :=
   match goal with
   | H : _, e : _ = _ |- _ => erewrite H by tac
   end.
+
+
+Definition rev {A} (l : list A) : list A :=
+  let fix aux (l : list A) (acc : list A) : list A :=
+    match l with
+    | [] => acc
+    | x :: l => aux l (x :: acc)
+    end
+  in aux l [].
+
+Definition rev_map {A B} (f : A -> B) (l : list A) : list B :=
+  let fix aux (l : list A) (acc : list B) : list B :=
+    match l with
+    | [] => acc
+    | x :: l => aux l (f x :: acc)
+    end
+  in aux l [].
